make lock spec a Class

iris_heap_lang/lib/lock.v
@@ -5,7 +5,7 @@ From iris.prelude Require Import options.
 (** A general interface for a lock.
 All parameters are implicit, since it is expected that there is only one
 [heapGS_gen] in scope that could possibly apply. *)
-Structure lock `{!heapGS_gen hlc Σ} := Lock {
+Class lock `{!heapGS_gen hlc Σ} := Lock {
   (** * Operations *)
   newlock : val;
   acquire : val;
@@ -18,11 +18,11 @@ Structure lock `{!heapGS_gen hlc Σ} := Lock {
   is_lock (γ: name) (lock: val) (R: iProp Σ) : iProp Σ;
   locked (γ: name) : iProp Σ;
   (** * General properties of the predicates *)
-  is_lock_ne γ lk : Contractive (is_lock γ lk);
-  is_lock_persistent γ lk R : Persistent (is_lock γ lk R);
+  is_lock_ne γ lk :> Contractive (is_lock γ lk);
+  is_lock_persistent γ lk R :> Persistent (is_lock γ lk R);
   is_lock_iff γ lk R1 R2 :
     is_lock γ lk R1 -∗ ▷ □ (R1 ↔ R2) -∗ is_lock γ lk R2;
-  locked_timeless γ : Timeless (locked γ);
+  locked_timeless γ :> Timeless (locked γ);
   locked_exclusive γ : locked γ -∗ locked γ -∗ False;
   (** * Program specs *)
   newlock_spec (R : iProp Σ) :
@@ -33,8 +33,6 @@ Structure lock `{!heapGS_gen hlc Σ} := Lock {
     {{{ is_lock γ lk R ∗ locked γ ∗ R }}} release lk {{{ RET #(); True }}}
 }.
 Global Hint Mode lock + + + : typeclass_instances.
-
-Global Existing Instances is_lock_ne is_lock_persistent locked_timeless.
 
 Global Instance is_lock_proper hlc Σ `{!heapGS_gen hlc Σ} (L : lock) γ lk :
   Proper ((≡) ==> (≡)) (L.(is_lock) γ lk) := ne_proper _.
